# 0003

<span></span>|<span></span>
:-: | :-:
$y = c_0 + c_1 x$ | $(1)$
$\displaystyle c_0 = \frac{y_1 x_2 - y_2 x_1}{x_2 - x_1}$ | $(2)$
$\displaystyle c_1 = \frac{y_2 - y_1}{x_2 - x_1}$ | $(3)$
<span></span>|<span></span>


## (4) & (5)
$$
\begin{array}{rcl}
y & = & f(x) \newline
& = & c_0 + c_1 x.
\end{array}
$$

$$\label{4}
y_1 = c_0 + c_1 x_1.
$$

$$\label{5}
y_2 = c_0 + c_1 x_2.
$$


## (2) = (7) &rightarrow; (5)
$$\tag{9}
\begin{array}{rcl}
y_2 & = & c_0 + \displaystyle \left( \frac{y_1 - y_2}{x_1 - x_2} \right) x_2 \newline
\displaystyle y_2 - \left( \frac{y_1 - y_2}{x_1 - x_2} \right) x_2 & = & c_0 \newline
\displaystyle \frac{y_2 x_1 - y_2 x_2 - y_1 x_2 + y_2 x_2}{x_1 - x_2} & = & \newline
\displaystyle \frac{y_2 x_1 - y_1 x_2}{x_1 - x_2} & = & \newline
c_0 & = & \displaystyle \frac{y_2 x_1 - y_1 x_2}{x_1 - x_2}.
\end{array}
$$


## (2) = (6) &rightarrow; (4)
$$\tag{8}
\begin{array}{rcl}
y_1 & = & c_0 + \displaystyle \left( \frac{y_2 - y_1}{x_2 - x_1} \right) x_1 \newline
\displaystyle y_1 - \left( \frac{y_2 - y_1}{x_2 - x_1} \right) x_1 & = & c_0 \newline
\displaystyle \frac{y_1 x_2 - y_1 x_1 - y_2 x_1 + y_1 x_1}{x_2 - x_1} & = & \newline
\displaystyle \frac{y_1 x_2 - y_2 x_1}{x_2 - x_1} & = & \newline
c_0 & = & \displaystyle \frac{y_1 x_2 - y_2 x_1}{x_2 - x_1}.
\end{array}
$$


## (3) = (4) - (5)
$$\tag{7}
\begin{array}{rcl}
y_1 - y_2 & = & c_1 (x_1 - x_2) \newline
\displaystyle \frac{y_1 - y_2}{x_1 - x_2} & = & c_1 \newline
c_1 & = & \displaystyle \frac{y_1 - y_2}{x_1 - x_2}.
\end{array}
$$


## (3) = (5) - (4)
$$\tag{6}
\begin{array}{rcl}
y_2 - y_1 & = & c_1 (x_2 - x_1) \newline
\displaystyle \frac{y_2 - y_1}{x_2 - x_1} & = & c_1 \newline
c_1 & = & \displaystyle \frac{y_2 - y_1}{x_2 - x_1}.
\end{array}
$$
