# 0011
```mermaid
graph LR
  %%
  %%linkStyle default fill:none,stroke-width:0px,stroke:none
  %%style Z1 stroke:none,fill:none;
  %%style Z2 width:0px,height:0px;
  %%linkStyle default fill:none,stroke-width:1px,stroke:lightgray;
  %%linkStyle 0 fill:none,stroke-width:0px,stroke:none;
``````

<span></span>|<span></span>
:-: | :-:
$\displaystyle \frac{\partial^2 \psi}{\partial x^2} - \frac{1}{v^2} \frac{\partial^2 \psi}{\partial t^2} = 0$ | $(1)$
$\psi(x, t) = X(x) T(t)$ | $(2)$
$\omega = kv$ | $(3)$
$\sin\alpha + \sin\beta = 2 \sin\tfrac12(\alpha + \beta) \cos\tfrac12(\alpha - \beta)$ | $(4)$
$\psi_A(x, t) = A \sin (kx + \omega t + \varphi_A)$ | $(5)$
$\psi_B(x, t) = B \sin (kx - \omega t + \varphi_B)$ | $(6)$
<span></span>|<span></span>


## (7) = (2) & (3) &rightarrow; (1)
$$
\begin{array}{rcl}
\displaystyle \frac{\partial^2}{\partial x^2} XT & = & \displaystyle \frac{1}{v^2} \frac{\partial^2}{\partial t^2} XT \newline
\displaystyle T \frac{\partial^2}{\partial x^2} X & = & \displaystyle X \frac{1}{v^2} \frac{\partial^2}{\partial t^2} T \newline
\displaystyle T \frac{d^2X}{dx^2} & = & \displaystyle X \frac{1}{v^2} \frac{d^2T}{dt^2} \newline
\displaystyle \frac{1}{X} \frac{d^2X}{dx^2} & = & \displaystyle \frac{1}{T} \frac{1}{v^2} \frac{d^2T}{dt^2} \newline
\displaystyle \frac{1}{X} \frac{d^2X}{dx^2} & = & -k^2 \newline
-k^2 & = & \displaystyle \frac{1}{T} \frac{1}{v^2} \frac{d^2T}{dt^2}
\end{array}
$$

### X
$$
\begin{array}{rcl}
\displaystyle \frac{1}{X} \frac{d^2X}{dx^2} & = & -k^2 \newline
\displaystyle \frac{d^2X}{dx^2} & = & -k^2 X \newline
X & = & S \sin (kx + \varphi_x)
\end{array}
$$

### T
$$
\begin{array}{rcl}
\displaystyle \frac{1}{T} \frac{1}{v^2} \frac{d^2T}{dt^2} & = & -k^2 \newline
\displaystyle \frac{d^2T}{dt^2} & = & -k^2 v^2 T \newline
& = & -\omega^2 T \newline
T & = & C \cos (\omega t + \varphi_t)
\end{array}
$$


## (4) &equiv; (7)
$$
\begin{array}{rcl}
\psi & = & (S \sin kx)(C \cos \omega t) \newline
& = & SC \sin (kx + \varphi_x) \cos (\omega t + \varphi_t)
\end{array}
$$

### &alpha;
$$
\begin{array}{rcl}
\tfrac12 (\alpha + \beta) & = & (kx + \varphi_x) \newline
\tfrac12 (\alpha - \beta) & = & (\omega t + \varphi_t) \newline
\alpha & = & kx + \omega t + \varphi_A
\end{array}
$$

### &beta;
$$
\begin{array}{rcl}
\tfrac12 (\alpha + \beta) & = & (kx + \varphi_x) \newline
\tfrac12 (\alpha - \beta) & = & (\omega t + \varphi_t) \newline
\beta & = & kx - \omega t + \varphi_B
\end{array}
$$


