# 0012
```mermaid
graph LR
  %%
  %%linkStyle default fill:none,stroke-width:0px,stroke:none
  %%style Z1 stroke:none,fill:none;
  %%style Z2 width:0px,height:0px;
  %%linkStyle default fill:none,stroke-width:1px,stroke:lightgray;
  %%linkStyle 0 fill:none,stroke-width:0px,stroke:none;
``````

<span></span>|<span></span>
:-: | :-:
$\displaystyle \frac{\partial^2 \psi}{\partial x^2} - \frac{1}{v^2} \frac{\partial^2 \psi}{\partial t^2} = 0$ | $(1)$
$\psi = \psi(x, t)$ | $(2)$
$\omega = kv$ | $(3)$
$\psi_1 = A \sin (kx + \omega t + \varphi_1)$ | $(4)$
$\psi_2 = B \cos (kx + \omega t + \varphi_2)$ | $(5)$
$\psi_3 = C \sin kx \cos(\omega t + \varphi_3)$ | $(6)$
$\psi_4 = D \sin kx \sin(\omega t + \varphi_4)$ | $(7)$
$\psi_5 = \psi_1 \pm \psi_2$ | $(8)$
$\psi_6 = \psi_3 \pm \psi_4$ | $(9)$
<span></span>|<span></span>


## (3) = (4) &rightarrow; (1)
$$
\begin{array}{rcl}
\displaystyle \frac{\partial^2}{\partial x^2} A \sin (kx + \omega t + \varphi_1) & = & \displaystyle \frac{1}{v^2} \frac{\partial^2}{\partial t^2} A \sin (kx + \omega t + \varphi_1) \newline
-k^2 A \sin (kx + \omega t + \varphi_1) & = & \displaystyle -\omega^2 \frac{1}{v^2} A \sin (kx + \omega t + \varphi_1) \newline
\displaystyle \left( -k^2 + \frac{\omega^2}{v^2} \right) A \sin (kx + \omega t + \varphi_1) & = & 0 \newline
k^2 & = & \displaystyle \frac{\omega^2}{v^2} \newline
k^2 v^2 & = & \omega^2 \newline
kv & = & \omega
\end{array}
$$
