# 0013
```mermaid
graph LR
  %%
```

<span></span>|<span></span>
:-: | :-:
$y_s(x, t) = y_+(x, t) + y_-(x, t)$ | $(1)$
$y_+(x, t) = A \sin (kx - \omega t)$ | $(2)$
$y_-(x, t) = A \sin (kx + \omega t)$ | $(3)$
$y_s(x, t) = B \sin kx \cos \omega t$ | $(4)$
<span></span>|<span></span>


## (4) = (2) & (3) &rightarrow; (1)
$$
\begin{array}{rcl}
y_s(x, t) & = & A \sin (kx - \omega t) + A \sin (kx + \omega t) \newline
& = & 2A \sin \tfrac12[(kx - \omega t) + (kx + \omega t)] \newline
& & \ \ \ \ \ \cos \tfrac12[(kx - \omega t) - (kx + \omega t)] \newline
& = & 2 A \sin kx \cos (-\omega t) \newline
& = & 2 A \sin kx \cos \omega t \newline
& = & B \sin kx \cos \omega t
\end{array}
$$
