# 0022
```mermaid
graph LR
  %%
```

<span></span>|<span></span>
:-: | :-:
$\displaystyle \frac{dy}{dx} = \frac{y_{i+1} - y_{i}}{h}$ | $(1)$
$\displaystyle \frac{dy}{dx} = \frac{y_{i} - y_{i-1}}{h}$ | $(2)$
$\displaystyle \frac{d^2y}{dx^2} = \frac{y_{i+1} - 2y_i + y_{i-1}}{h^2}$ | $(3)$
$\displaystyle \frac{d^2y}{dt^2} = -g$ | $(4)$
$\displaystyle \frac{dy}{dt} = v$ | $(5)$
$N = 10$ | $(6)$
$h = 0.5$ | $(7)$
$y_i = y_0 + ih, \ \ \ \ i = 0, \dots, N$ | $(8)$
$v(t_0) = v_0$ | $(9)$
$v(t_N) = v_N$ | $(10)$
<span></span>|<span></span>


## (17) = (16)<sup>-1</sup>
$$
\left[
\begin{array}{c}
y_0 \newline
y_1 \newline
y_2 \newline
y_3 \newline
y_4 \newline
y_5 \newline
y_6 \newline
y_7 \newline
y_8 \newline
y_9 \newline
y_{10}
\end{array}
\right] =
\left[
\begin{array}{ccccccccccc}
-1 &  1 &  0 &  0 &  0 &  0 &  0 &  0 &  0 &  0 &  0 \newline 
 1 & -2 &  1 &  0 &  0 &  0 &  0 &  0 &  0 &  0 &  0 \newline 
 0 &  1 & -2 &  1 &  0 &  0 &  0 &  0 &  0 &  0 &  0 \newline 
 0 &  0 &  1 & -2 &  1 &  0 &  0 &  0 &  0 &  0 &  0 \newline 
 0 &  0 &  0 &  1 & -2 &  1 &  0 &  0 &  0 &  0 &  0 \newline 
 0 &  0 &  0 &  0 &  1 & -2 &  1 &  0 &  0 &  0 &  0 \newline 
 0 &  0 &  0 &  0 &  0 &  1 & -2 &  1 &  0 &  0 &  0 \newline 
 0 &  0 &  0 &  0 &  0 &  0 &  1 & -2 &  1 &  0 &  0 \newline 
 0 &  0 &  0 &  0 &  0 &  0 &  0 &  1 & -2 &  1 &  0 \newline 
 0 &  0 &  0 &  0 &  0 &  0 &  0 &  0 &  1 & -2 &  1 \newline 
 0 &  0 &  0 &  0 &  0 &  0 &  0 &  0 &  0 & -1 &  1 \newline 
\end{array}
\right]^{-1}
\left[ \begin{array}{c}
h v(t_0) \newline
-gh^2 \newline
-gh^2 \newline
-gh^2 \newline
-gh^2 \newline
-gh^2 \newline
-gh^2 \newline
-gh^2 \newline
-gh^2 \newline
-gh^2 \newline
h v(t_N)
\end{array}
\right]
$$


## (16) = (8) & (14) & (15) 
$$
\left[
\begin{array}{ccccccccccc}
-1 &  1 &  0 &  0 &  0 &  0 &  0 &  0 &  0 &  0 &  0 \newline 
 1 & -2 &  1 &  0 &  0 &  0 &  0 &  0 &  0 &  0 &  0 \newline 
 0 &  1 & -2 &  1 &  0 &  0 &  0 &  0 &  0 &  0 &  0 \newline 
 0 &  0 &  1 & -2 &  1 &  0 &  0 &  0 &  0 &  0 &  0 \newline 
 0 &  0 &  0 &  1 & -2 &  1 &  0 &  0 &  0 &  0 &  0 \newline 
 0 &  0 &  0 &  0 &  1 & -2 &  1 &  0 &  0 &  0 &  0 \newline 
 0 &  0 &  0 &  0 &  0 &  1 & -2 &  1 &  0 &  0 &  0 \newline 
 0 &  0 &  0 &  0 &  0 &  0 &  1 & -2 &  1 &  0 &  0 \newline 
 0 &  0 &  0 &  0 &  0 &  0 &  0 &  1 & -2 &  1 &  0 \newline 
 0 &  0 &  0 &  0 &  0 &  0 &  0 &  0 &  1 & -2 &  1 \newline 
 0 &  0 &  0 &  0 &  0 &  0 &  0 &  0 &  0 & -1 &  1 \newline 
\end{array}
\right]
\left[
\begin{array}{c}
y_0 \newline
y_1 \newline
y_2 \newline
y_3 \newline
y_4 \newline
y_5 \newline
y_6 \newline
y_7 \newline
y_8 \newline
y_9 \newline
y_{10}
\end{array}
\right] =
\left[ \begin{array}{c}
h v(t_0) \newline
-gh^2 \newline
-gh^2 \newline
-gh^2 \newline
-gh^2 \newline
-gh^2 \newline
-gh^2 \newline
-gh^2 \newline
-gh^2 \newline
-gh^2 \newline
h v(t_N)
\end{array}
\right]
$$


## (15) = (10) &rightarrow; (13)
$$
y_{11} - y_{10} = h v(t_N)
$$


## (14) = (9) &rightarrow; (12)
$$
y_1 - y_0 = h v(t_0)
$$


## (13) = (2) &rightarrow; (5)
$$
\begin{array}{rcl}
\displaystyle \frac{y_{i} - y_{i-1}}{h} & = & v \newline
y_{i} - y_{i-1} & = & h v
\end{array}
$$


## (12) = (1) &rightarrow; (5)
$$
\begin{array}{rcl}
\displaystyle \frac{y_{i+1} - y_{i}}{h} & = & v \newline
y_{i+1} - y_{i} & = & h v
\end{array}
$$


## (11) = (2) &rightarrow; (3)
$$
\begin{array}{rcl}
\displaystyle \frac{y_{i+1} - 2y_i + y_{i-1}}{h^2} & = & -g \newline
y_{i+1} - 2y_i + y_{i-1} & = & -gh^2
\end{array}
$$


## refs
+ "Finite Difference Method", url <https://pythonnumericalmethods.berkeley.edu/notebooks/chapter23.03-Finite-Difference-Method.html> [20221025].
+ "5 Types Of Boundary Conditions In Mathematics And Sciences - Education - Nairaland", url <https://www.nairaland.com/3055062/5-types-boundary-conditions-mathematics> [20221025].